books/projects/async/gcd/gcd2.lisp
@@ -181,10 +181,10 @@
 ;; Constraints on the state of GCD2
 
 (defund gcd2$st-format (st data-size)
-  (b* ((l0 (get-field *gcd2$l0* st))
-       (l1 (get-field *gcd2$l1* st))
-       (l2 (get-field *gcd2$l2* st))
-       (body (get-field *gcd2$body* st)))
+  (b* ((l0 (nth *gcd2$l0* st))
+       (l1 (nth *gcd2$l1* st))
+       (l2 (nth *gcd2$l2* st))
+       (body (nth *gcd2$body* st)))
     (and (<= 3 data-size)
          (link$st-format l0 (* 2 data-size))
          (link$st-format l1 (* 2 data-size))
@@ -199,11 +199,11 @@
   :rule-classes :forward-chaining)
 
 (defund gcd2$valid-st (st data-size)
-  (b* ((s  (get-field *gcd2$s* st))
-       (l0 (get-field *gcd2$l0* st))
-       (l1 (get-field *gcd2$l1* st))
-       (l2 (get-field *gcd2$l2* st))
-       (body (get-field *gcd2$body* st)))
+  (b* ((s  (nth *gcd2$s* st))
+       (l0 (nth *gcd2$l0* st))
+       (l1 (nth *gcd2$l1* st))
+       (l2 (nth *gcd2$l2* st))
+       (body (nth *gcd2$body* st)))
     (and (<= 3 data-size)
          (link1$valid-st s)
          (link$valid-st l0 (* 2 data-size))
@@ -254,14 +254,14 @@
 
          (me-go-signals (take *merge$go-num* go-signals))
 
-         (s (get-field *gcd2$s* st))
-         (s.s (get-field *link1$s* s))
-         (s.d (get-field *link1$d* s))
-         (l0 (get-field *gcd2$l0* st))
-         (l0.s (get-field *link$s* l0))
-         (l2 (get-field *gcd2$l2* st))
-         (l2.s (get-field *link$s* l2))
-         (l2.d (get-field *link$d* l2))
+         (s (nth *gcd2$s* st))
+         (s.s (nth *link1$s* s))
+         (s.d (nth *link1$d* s))
+         (l0 (nth *gcd2$l0* st))
+         (l0.s (nth *link$s* l0))
+         (l2 (nth *gcd2$l2* st))
+         (l2.s (nth *link$s* l2))
+         (l2.d (nth *link$d* l2))
 
          (me-full-in0 (f-and full-in (car s.s)))
          (me-full-in1 (f-and (car l2.s) (car s.s))))
@@ -280,13 +280,13 @@
          (br-go-signals (take *gcd-cond$go-num*
                               (nthcdr *merge$go-num* go-signals)))
 
-         (s (get-field *gcd2$s* st))
-         (s.s (get-field *link1$s* s))
-         (l0 (get-field *gcd2$l0* st))
-         (l0.s (get-field *link$s* l0))
-         (l0.d (get-field *link$d* l0))
-         (l1 (get-field *gcd2$l1* st))
-         (l1.s (get-field *link$s* l1))
+         (s (nth *gcd2$s* st))
+         (s.s (nth *link1$s* s))
+         (l0 (nth *gcd2$l0* st))
+         (l0.s (nth *link$s* l0))
+         (l0.d (nth *link$d* l0))
+         (l1 (nth *gcd2$l1* st))
+         (l1.s (nth *link$s* l1))
 
          (br-empty-out0- (f-or empty-out- (car s.s)))
          (br-empty-out1- (f-or (car l1.s) (car s.s))))
@@ -305,11 +305,11 @@
                                            *gcd-cond$go-num*)
                                         go-signals)))
 
-         (l1 (get-field *gcd2$l1* st))
-         (l1.s (get-field *link$s* l1))
-         (l1.d (get-field *link$d* l1))
-         (l2 (get-field *gcd2$l2* st))
-         (l2.s (get-field *link$s* l2)))
+         (l1 (nth *gcd2$l1* st))
+         (l1.s (nth *link$s* l1))
+         (l1.d (nth *link$d* l1))
+         (l2 (nth *gcd2$l2* st))
+         (l2.s (nth *link$s* l2)))
 
       (list* (f-buf (car l1.s)) (f-buf (car l2.s))
              (append (v-threefix (strip-cars l1.d))
@@ -413,13 +413,13 @@
 (defun gcd2$step (inputs st data-size)
   (b* ((data-in (gcd2$data-in inputs data-size))
 
-       (s (get-field *gcd2$s* st))
-       (s.d (get-field *link1$d* s))
-       (l0 (get-field *gcd2$l0* st))
-       (l1 (get-field *gcd2$l1* st))
-       (l2 (get-field *gcd2$l2* st))
-       (l2.d (get-field *link$d* l2))
-       (body (get-field *gcd2$body* st))
+       (s (nth *gcd2$s* st))
+       (s.d (nth *link1$d* s))
+       (l0 (nth *gcd2$l0* st))
+       (l1 (nth *gcd2$l1* st))
+       (l2 (nth *gcd2$l2* st))
+       (l2.d (nth *link$d* l2))
+       (body (nth *gcd2$body* st))
 
        (me-inputs (gcd2$me-inputs inputs st data-size))
        (br-inputs (gcd2$br-inputs inputs st data-size))
@@ -559,10 +559,10 @@
 ;; sequence from the current state.
 
 (defund gcd2$extract (st data-size)
-  (b* ((l0 (get-field *gcd2$l0* st))
-       (l1 (get-field *gcd2$l1* st))
-       (l2 (get-field *gcd2$l2* st))
-       (body (get-field *gcd2$body* st)))
+  (b* ((l0 (nth *gcd2$l0* st))
+       (l1 (nth *gcd2$l1* st))
+       (l2 (nth *gcd2$l2* st))
+       (body (nth *gcd2$body* st)))
     (gcd$op-map
      (append (extract-valid-data (list l0 l1 l2))
              (gcd-body2$extract body data-size)))))
@@ -586,10 +586,10 @@
 
 (progn
   (defund gcd2$inv (st data-size)
-    (b* ((s (get-field *gcd2$s* st))
-         (s.s (get-field *link1$s* s))
-         (s.d (get-field *link1$d* s))
-         (body (get-field *gcd2$body* st)))
+    (b* ((s (nth *gcd2$s* st))
+         (s.s (nth *link1$s* s))
+         (s.d (nth *link1$d* s))
+         (body (nth *gcd2$body* st)))
       (and (if (and (fullp s.s) (not (car s.d)))
                (= (len (gcd2$extract st data-size))
                   0)
@@ -626,8 +626,7 @@
           (body (nth *gcd2$body* st)))
        (implies (emptyp l1.s)
                 (not (gcd-body2$in-act body-inputs body data-size))))
-     :hints (("Goal" :in-theory (enable get-field
-                                        gcd2$body-inputs)))))
+     :hints (("Goal" :in-theory (enable gcd2$body-inputs)))))
 
   (defthm gcd2$inv-preserved
     (implies (and (gcd2$input-format inputs data-size)
@@ -637,8 +636,7 @@
                            data-size))
     :hints (("Goal"
              :use gcd2$input-format=>body$input-format
-             :in-theory (e/d (get-field
-                              f-sr
+             :in-theory (e/d (f-sr
                               gcd-body2$extracted-step
                               gcd2$valid-st
                               gcd2$inv
@@ -707,8 +705,7 @@
                      (equal (len l1.d) (* 2 data-size)))
                 (equal (gcd-body2$data-in body-inputs data-size)
                        (v-threefix (strip-cars l1.d)))))
-     :hints (("Goal" :in-theory (enable get-field
-                                        gcd-body2$data-in
+     :hints (("Goal" :in-theory (enable gcd-body2$data-in
                                         gcd2$body-inputs)))))
 
   (local
@@ -733,8 +730,7 @@
                       (gcd2$extracted-step inputs st data-size))))
     :hints (("Goal"
              :use gcd2$input-format=>body$input-format
-             :in-theory (e/d (get-field
-                              f-sr
+             :in-theory (e/d (f-sr
                               joint-act
                               fv-if-rewrite
                               gcd-body2$valid-st=>constraint
@@ -782,8 +778,7 @@
           (body (nth *gcd2$body* st)))
        (implies (fullp l2.s)
                 (not (gcd-body2$out-act body-inputs body data-size))))
-     :hints (("Goal" :in-theory (enable get-field
-                                        gcd2$body-inputs)))))
+     :hints (("Goal" :in-theory (enable gcd2$body-inputs)))))
 
   (defthm gcd2$valid-st-preserved
     (implies (and (gcd2$input-format inputs data-size)
@@ -793,8 +788,7 @@
               data-size))
     :hints (("Goal"
              :use gcd2$input-format=>body$input-format
-             :in-theory (e/d (get-field
-                              f-sr
+             :in-theory (e/d (f-sr
                               joint-act
                               gcd-body2$valid-st=>constraint
                               gcd2$valid-st
