books/projects/async/serial-adder/piso-sreg.lisp
@@ -216,10 +216,10 @@
 ;; Constraints on the state of PISO-SREG
 
 (defund piso-sreg$st-format (st data-size cnt-size)
-  (b* ((r-data (get-field *piso-sreg$r-data* st))
-       (r-cnt (get-field *piso-sreg$r-cnt* st))
-       (w-data (get-field *piso-sreg$w-data* st))
-       (w-cnt (get-field *piso-sreg$w-cnt* st)))
+  (b* ((r-data (nth *piso-sreg$r-data* st))
+       (r-cnt (nth *piso-sreg$r-cnt* st))
+       (w-data (nth *piso-sreg$w-data* st))
+       (w-cnt (nth *piso-sreg$w-cnt* st)))
     (and (posp data-size)
          (natp cnt-size)
          (<= 3 cnt-size)
@@ -237,10 +237,10 @@
   :rule-classes :forward-chaining)
 
 (defund piso-sreg$valid-st (st data-size cnt-size)
-  (b* ((r-data (get-field *piso-sreg$r-data* st))
-       (r-cnt (get-field *piso-sreg$r-cnt* st))
-       (w-data (get-field *piso-sreg$w-data* st))
-       (w-cnt (get-field *piso-sreg$w-cnt* st)))
+  (b* ((r-data (nth *piso-sreg$r-data* st))
+       (r-cnt (nth *piso-sreg$r-cnt* st))
+       (w-data (nth *piso-sreg$w-data* st))
+       (w-cnt (nth *piso-sreg$w-cnt* st)))
     (and (piso-sreg$st-format st data-size cnt-size)
          (equal data-size (expt 2 (1- cnt-size)))
          (link$valid-st r-data data-size)
@@ -295,15 +295,15 @@
                              inputs))
          (go-shift (nth 0 go-signals))
 
-         (r-data (get-field *piso-sreg$r-data* st))
-         (r-data.s (get-field *link$s* r-data))
-         (r-cnt (get-field *piso-sreg$r-cnt* st))
-         (r-cnt.s (get-field *link$s* r-cnt))
-         (r-cnt.d (get-field *link$d* r-cnt))
-         (w-data (get-field *piso-sreg$w-data* st))
-         (w-data.s (get-field *link$s* w-data))
-         (w-cnt (get-field *piso-sreg$w-cnt* st))
-         (w-cnt.s (get-field *link$s* w-cnt))
+         (r-data (nth *piso-sreg$r-data* st))
+         (r-data.s (nth *link$s* r-data))
+         (r-cnt (nth *piso-sreg$r-cnt* st))
+         (r-cnt.s (nth *link$s* r-cnt))
+         (r-cnt.d (nth *link$d* r-cnt))
+         (w-data (nth *piso-sreg$w-data* st))
+         (w-data.s (nth *link$s* w-data))
+         (w-cnt (nth *piso-sreg$w-cnt* st))
+         (w-cnt.s (nth *link$s* w-cnt))
 
          (r-cnt=0 (f$fast-zero (strip-cars r-cnt.d)))
          (shift-full-in (f-and4 (car r-data.s) (car r-cnt.s)
@@ -325,15 +325,15 @@
                              inputs))
          (go-shift (nth 0 go-signals))
 
-         (r-data (get-field *piso-sreg$r-data* st))
-         (r-data.s (get-field *link$s* r-data))
-         (r-cnt (get-field *piso-sreg$r-cnt* st))
-         (r-cnt.s (get-field *link$s* r-cnt))
-         (r-cnt.d (get-field *link$d* r-cnt))
-         (w-data (get-field *piso-sreg$w-data* st))
-         (w-data.s (get-field *link$s* w-data))
-         (w-cnt (get-field *piso-sreg$w-cnt* st))
-         (w-cnt.s (get-field *link$s* w-cnt))
+         (r-data (nth *piso-sreg$r-data* st))
+         (r-data.s (nth *link$s* r-data))
+         (r-cnt (nth *piso-sreg$r-cnt* st))
+         (r-cnt.s (nth *link$s* r-cnt))
+         (r-cnt.d (nth *link$d* r-cnt))
+         (w-data (nth *piso-sreg$w-data* st))
+         (w-data.s (nth *link$s* w-data))
+         (w-cnt (nth *piso-sreg$w-cnt* st))
+         (w-cnt.s (nth *link$s* w-cnt))
 
          (r-cnt=0~ (f-not (f$fast-zero (strip-cars r-cnt.d))))
          (r-full (f-and3 (car r-data.s) (car r-cnt.s) r-cnt=0~))
@@ -358,8 +358,8 @@
   ;; Extract the output data
 
   (defund piso-sreg$bit-out (st)
-    (b* ((r-data (get-field *piso-sreg$r-data* st))
-         (r-data.d (get-field *link$d* r-data)))
+    (b* ((r-data (nth *piso-sreg$r-data* st))
+         (r-data.d (nth *link$d* r-data)))
       (f-buf (car (strip-cars r-data.d)))))
 
   (defthm booleanp-piso-sreg$bit-out
@@ -415,18 +415,18 @@
                            inputs))
        (go-buf   (nth 1 go-signals))
 
-       (r-data (get-field *piso-sreg$r-data* st))
-       (r-data.s (get-field *link$s* r-data))
-       (r-data.d (get-field *link$d* r-data))
-       (r-cnt (get-field *piso-sreg$r-cnt* st))
-       (r-cnt.s (get-field *link$s* r-cnt))
-       (r-cnt.d (get-field *link$d* r-cnt))
-       (w-data (get-field *piso-sreg$w-data* st))
-       (w-data.s (get-field *link$s* w-data))
-       (w-data.d (get-field *link$d* w-data))
-       (w-cnt (get-field *piso-sreg$w-cnt* st))
-       (w-cnt.s (get-field *link$s* w-cnt))
-       (w-cnt.d (get-field *link$d* w-cnt))
+       (r-data (nth *piso-sreg$r-data* st))
+       (r-data.s (nth *link$s* r-data))
+       (r-data.d (nth *link$d* r-data))
+       (r-cnt (nth *piso-sreg$r-cnt* st))
+       (r-cnt.s (nth *link$s* r-cnt))
+       (r-cnt.d (nth *link$d* r-cnt))
+       (w-data (nth *piso-sreg$w-data* st))
+       (w-data.s (nth *link$s* w-data))
+       (w-data.d (nth *link$d* w-data))
+       (w-cnt (nth *piso-sreg$w-cnt* st))
+       (w-cnt.s (nth *link$s* w-cnt))
+       (w-cnt.d (nth *link$d* w-cnt))
 
        (r-cnt=0 (f$fast-zero (strip-cars r-cnt.d)))
        (in-act (piso-sreg$in-act inputs st data-size))
@@ -581,15 +581,15 @@
 ;; The extraction function for PISO-SREG
 
 (defund piso-sreg$extract (st)
-  (b* ((r-data (get-field *piso-sreg$r-data* st))
-       (r-data.s (get-field *link$s* r-data))
-       (r-data.d (get-field *link$d* r-data))
-       (r-cnt (get-field *piso-sreg$r-cnt* st))
-       (r-cnt.d (get-field *link$d* r-cnt))
-       (w-data (get-field *piso-sreg$w-data* st))
-       (w-data.d (get-field *link$d* w-data))
-       (w-cnt (get-field *piso-sreg$w-cnt* st))
-       (w-cnt.d (get-field *link$d* w-cnt)))
+  (b* ((r-data (nth *piso-sreg$r-data* st))
+       (r-data.s (nth *link$s* r-data))
+       (r-data.d (nth *link$d* r-data))
+       (r-cnt (nth *piso-sreg$r-cnt* st))
+       (r-cnt.d (nth *link$d* r-cnt))
+       (w-data (nth *piso-sreg$w-data* st))
+       (w-data.d (nth *link$d* w-data))
+       (w-cnt (nth *piso-sreg$w-cnt* st))
+       (w-cnt.d (nth *link$d* w-cnt)))
     (if (fullp r-data.s)
         (take (v-to-nat (strip-cars r-cnt.d))
               (strip-cars r-data.d))
@@ -650,18 +650,18 @@
 
 (progn
   (defund piso-sreg$inv (st)
-    (b* ((r-data (get-field *piso-sreg$r-data* st))
-         (r-data.s (get-field *link$s* r-data))
-         (r-data.d (get-field *link$d* r-data))
-         (r-cnt (get-field *piso-sreg$r-cnt* st))
-         (r-cnt.s (get-field *link$s* r-cnt))
-         (r-cnt.d (get-field *link$d* r-cnt))
-         (w-data (get-field *piso-sreg$w-data* st))
-         (w-data.s (get-field *link$s* w-data))
-         (w-data.d (get-field *link$d* w-data))
-         (w-cnt (get-field *piso-sreg$w-cnt* st))
-         (w-cnt.s (get-field *link$s* w-cnt))
-         (w-cnt.d (get-field *link$d* w-cnt)))
+    (b* ((r-data (nth *piso-sreg$r-data* st))
+         (r-data.s (nth *link$s* r-data))
+         (r-data.d (nth *link$d* r-data))
+         (r-cnt (nth *piso-sreg$r-cnt* st))
+         (r-cnt.s (nth *link$s* r-cnt))
+         (r-cnt.d (nth *link$d* r-cnt))
+         (w-data (nth *piso-sreg$w-data* st))
+         (w-data.s (nth *link$s* w-data))
+         (w-data.d (nth *link$d* w-data))
+         (w-cnt (nth *piso-sreg$w-cnt* st))
+         (w-cnt.s (nth *link$s* w-cnt))
+         (w-cnt.d (nth *link$d* w-cnt)))
       (and (equal r-data.s r-cnt.s)
            (equal w-data.s w-cnt.s)
            (not (equal r-data.s w-data.s))
@@ -718,8 +718,7 @@
              (piso-sreg$inv
               (piso-sreg$step inputs st data-size cnt-size)))
     :hints (("Goal"
-             :in-theory (e/d (get-field
-                              f-sr
+             :in-theory (e/d (f-sr
                               bvp
                               pos-len=>cons
                               piso-sreg$valid-st
@@ -753,8 +752,7 @@
              (equal (piso-sreg$extract next-st)
                     (piso-sreg$extracted-step inputs st data-size))))
   :hints (("Goal"
-           :in-theory (e/d (get-field
-                            f-sr
+           :in-theory (e/d (f-sr
                             joint-act
                             bvp
                             pos-len=>cons
@@ -781,8 +779,7 @@
             data-size
             cnt-size))
   :hints (("Goal"
-           :in-theory (e/d (get-field
-                            f-sr
+           :in-theory (e/d (f-sr
                             joint-act
                             bvp
                             f-and3
